proofs/proofsystem/Compat.v
@@ -1,0 +1,875 @@
+(*The stdpp versions of sets and maps are nice for proofs (extensional) but bad
+  for computation (the positives are VERY large) and slow the proof system down
+  substantially.
+  Here, we redefine some of the transformations using the old list-based versions.
+  We prove equivalence with the gmap-based versions and then rewrite to these in
+  the tactics in Tactics.v
+  substitution and free variable computations are the main culprit for slowdowns.
+  anything occurring in an "if" expression is fine: we can vm_compute to a bool anyway*)
+From Proofs Require Import Task SubMulti Alpha.
+From Proofs Require MatchSimpl Rewrite.
+Set Bullet Behavior "Strict Subproofs".
+
+Lemma amap_lookup_list {A B: Type} `{countable.Countable A} (l: list (A * B)) (x: A):
+  amap_lookup (list_to_amap l) x =
+  get_assoc_list EqDecision0 l x.
+Proof.
+  induction l as [| h t IH]; simpl.
+  - apply amap_empty_get.
+  - destruct (EqDecision0 x (fst h)); subst; simpl.
+    + apply amap_set_lookup_same.
+    + rewrite amap_set_lookup_diff; auto.
+Qed.
+
+(* list set ops *)
+
+Section ListSet.
+
+Context {A: Type}.
+Variable eq_dec: forall (x y : A), {x = y} + {x <> y}.
+
+(*Add all elements in l1 not in l2*)
+Definition union (l1 l2: list A) :=
+    fold_right (fun x acc => if in_dec eq_dec x acc then acc else x :: acc) l2 l1.
+
+(*Iterated union*)
+Definition big_union {B: Type} (f: B -> list A) (l: list B) :=
+  fold_right (fun x acc => union (f x) acc) nil l.
+
+Definition remove_all (l1 l2: list A) :=
+  fold_right (remove eq_dec) l2 l1.
+
+Lemma union_elts (l1 l2: list A) (x: A):
+  In x (union l1 l2) <-> In x l1 \/ In x l2.
+Proof.
+  induction l1; simpl; auto.
+  - split; intros; auto. destruct H as [[] |]; auto.
+  - split; intros Hin; destruct (in_dec eq_dec a (union l1 l2)).
+    + apply IHl1 in Hin. destruct Hin; solve_or.
+    + destruct Hin; subst; try solve_or. apply IHl1 in H; destruct H; solve_or.
+    + apply IHl1. destruct Hin as [Hin |?]; [destruct Hin; subst |]; try solve_or.
+      apply IHl1; auto.
+    + simpl. destruct Hin as [Hin|?]; [destruct Hin; subst|]; try solve_or.
+      all: right; apply IHl1; solve_or.
+Qed.
+
+(*relate sets and lists - lift to aset so we have ext*)
+
+Lemma union_list `{countable.Countable A} s1 s2:
+  aset_union (list_to_aset s1) (list_to_aset s2) =
+  list_to_aset (union s1 s2).
+Proof.
+  apply aset_ext. intros x. simpl_set. rewrite union_elts. reflexivity.
+Qed.
+
+Lemma singleton_list `{countable.Countable A} (x: A):
+  aset_singleton x = list_to_aset [x].
+Proof.
+  apply aset_ext. intros y. simpl_set. simpl. 
+  split; intros; destruct_all; auto. contradiction.
+Qed.
+
+End ListSet.
+
+
+Section Maps.
+(*Relate maps and assoc lists*)
+Lemma amap_singleton_list {A B: Type} `{countable.Countable A} (x: A) (y: B):
+  amap_singleton x y = list_to_amap [(x, y)].
+Proof.
+  reflexivity.
+Qed.
+
+Lemma amap_union_list {A B: Type} `{countable.Countable A} (l1 l2: list (A * B)):
+  list_to_amap (l1 ++ l2) = aunion (list_to_amap l1) (list_to_amap l2).
+Proof.
+  apply amap_ext. intros x. rewrite aunion_lookup.
+  rewrite !amap_lookup_list.
+  induction l1 as [| [x1 y1] t1]; simpl; auto.
+  destruct (EqDecision0 x x1); subst; auto.
+Qed.
+
+
+Lemma in_remove_iff {A} eq_dec
+  (y : A) (l: list A) (x: A):
+  In x (remove eq_dec y l) <-> In x l /\ x <> y.
+Proof.
+  split; intros.
+  - apply (in_remove eq_dec _ _ _ H).
+  - apply in_in_remove; apply H.
+Qed.
+
+Lemma remove_all_elts {A} eq_dec
+(l1 l2: list A) x:
+(In x l2 /\ ~In x l1) <-> In x (remove_all eq_dec l1 l2).
+Proof.
+  induction l1; simpl; split; intros; auto.
+  destruct H; auto.
+  - destruct H as [Hinx Hnot].
+    destruct (eq_dec x a); subst; auto.
+    + exfalso. apply Hnot; left; auto.
+    + rewrite in_remove_iff, <- IHl1. split_all; auto.
+  - rewrite in_remove_iff in H. destruct H.
+    apply IHl1 in H. split_all; auto.
+    intro C. destruct C; subst; contradiction.
+Qed.
+
+Lemma remove_list {A: Type} `{countable.Countable A} eq_dec (l: list A) x:
+  aset_remove x (list_to_aset l) = list_to_aset (remove eq_dec x l).
+Proof.
+  apply aset_ext. intros y. simpl_set. split.
+  - intros [Hin Hneq]. apply in_in_remove; auto.
+  - apply in_remove.
+Qed.
+
+Lemma diff_list {A: Type} `{countable.Countable A} eq_dec (l1 l2: list A):
+  aset_diff (list_to_aset l1) (list_to_aset l2) =
+  list_to_aset (remove_all eq_dec l1 l2).
+Proof.
+  apply aset_ext. intros x. simpl_set. apply remove_all_elts.
+Qed.
+End Maps.
+
+(*free vars*)
+Section Fv.
+
+Local Notation union' := (union vsymbol_eq_dec).
+Local Notation big_union' := (big_union vsymbol_eq_dec).
+Local Notation remove' := (remove vsymbol_eq_dec).
+Local Notation remove_all' := (remove_all vsymbol_eq_dec).
+
+(*Free variables of a pattern*)
+Fixpoint pat_fv' (p: pattern) : list vsymbol :=
+  match p with
+  | Pvar x => [x]
+  | Pwild => []
+  | Pconstr _ _ ps => big_union' pat_fv' ps
+  | Por p1 p2 => union' (pat_fv' p1) (pat_fv' p2)
+  | Pbind p x => union' (pat_fv' p) [x]
+  end.
+
+(*Free variables of a term (all variables that appear free at least once)*)
+Fixpoint tm_fv' (t: term) : list vsymbol :=
+  match t with
+  | Tconst _ => nil
+  | Tvar x => [x]
+  | Tfun f vtys tms => big_union' tm_fv' tms
+  | Tlet t1 v t2 => union' (tm_fv' t1) (remove' v (tm_fv' t2))
+  | Tif f t1 t2 => union' (fmla_fv' f) (union' (tm_fv' t1) (tm_fv' t2))
+  | Tmatch t ty l => union' (tm_fv' t) (big_union' (fun x => remove_all' (pat_fv' (fst x)) (tm_fv' (snd x))) l)
+  | Teps f x  => remove' x (fmla_fv' f)
+  end
+
+with fmla_fv' (f: formula) : list vsymbol :=
+  match f with
+  | Fpred p tys tms => big_union' tm_fv' tms
+  | Fquant q v f => remove' v (fmla_fv' f)
+  | Feq _ t1 t2 => union' (tm_fv' t1) (tm_fv' t2)
+  | Fbinop b f1 f2 => union' (fmla_fv' f1) (fmla_fv' f2)
+  | Fnot f => fmla_fv' f
+  | Ftrue => nil
+  | Ffalse => nil
+  | Flet t v f => union' (tm_fv' t) (remove' v (fmla_fv' f))
+  | Fif f1 f2 f3 => union' (fmla_fv' f1) (union' (fmla_fv' f2) (fmla_fv' f3))
+  | Fmatch t ty l => union' (tm_fv' t) (big_union' (fun x => remove_all' (pat_fv' (fst x)) (fmla_fv' (snd x))) l)
+  end.
+
+
+Lemma pat_fv_list p:
+  pat_fv p = list_to_aset (pat_fv' p).
+Proof.
+  induction p as [v | f tys tms IH | | p1 p2 IH1 IH2 | v p IH]; simpl.
+  - apply singleton_list.
+  - induction tms as [| h t IHtms]; simpl; auto.
+    inversion IH as [| ? ? IH1 IH2]; subst.
+    rewrite IH1. rewrite IHtms; auto.
+    (*NOTE: could have lemma for big_union, see*)
+    apply union_list.
+  - reflexivity.
+  - rewrite -> IH1, IH2. apply union_list.
+  - rewrite -> IH, singleton_list. apply union_list.
+Qed.
+
+
+Lemma fv_list t f:
+  (tm_fv t = list_to_aset (tm_fv' t)) /\ (fmla_fv f = list_to_aset (fmla_fv' f)).
+Proof.
+  revert t f;
+  apply term_formula_ind; simpl; auto; try reflexivity.
+  - intros v. rewrite singleton_list; auto.
+  - intros _ _ tms IH.
+    induction tms as [| h t IHtm]; simpl; auto.
+    inversion IH as [| ? ? IH1 IH2]; subst. rewrite IH1, IHtm; auto.
+    apply union_list.
+  - intros tm1 v tm2 IH1 IH2. rewrite IH1, IH2. rewrite <- union_list. f_equal.
+    apply remove_list.
+  - intros f t1 t2 IH1 IH2 IH3. rewrite IH1, IH2, IH3.
+    rewrite <- union_list; f_equal; apply union_list.
+  - intros tm _ ps IH1 IH2. rewrite IH1. rewrite <- union_list; f_equal. clear IH1.
+    rewrite Forall_map in IH2. induction ps as [| p1 ptl IH]; simpl; auto.
+    inversion IH2 as [| ? ? IHp1 IHtl]; subst; clear IH2. rewrite IHp1, IH; auto.
+    rewrite <- union_list, pat_fv_list. f_equal. apply diff_list.
+  - intros f v IH. rewrite IH. apply remove_list.
+  - intros _ _ tms IH.
+    induction tms as [| h t IHtm]; simpl; auto.
+    inversion IH as [| ? ? IH1 IH2]; subst. rewrite IH1, IHtm; auto.
+    apply union_list.
+  - intros _ v f IH.  rewrite IH. apply remove_list.
+  - intros _ t1 t2 IH1 IH2. rewrite IH1, IH2; apply union_list.
+  - intros _ t1 t2 IH1 IH2. rewrite IH1, IH2; apply union_list.
+  - intros tm1 v tm2 IH1 IH2. rewrite IH1, IH2. rewrite <- union_list. f_equal.
+    apply remove_list.
+  - intros ? ? ? IH1 IH2 IH3. rewrite IH1, IH2, IH3.
+    rewrite <- union_list; f_equal; apply union_list.
+  - intros tm _ ps IH1 IH2. rewrite IH1. rewrite <- union_list; f_equal. clear IH1.
+    rewrite Forall_map in IH2. induction ps as [| p1 ptl IH]; simpl; auto.
+    inversion IH2 as [| ? ? IHp1 IHtl]; subst; clear IH2. rewrite IHp1, IH; auto.
+    rewrite <- union_list, pat_fv_list. f_equal. apply diff_list.
+Qed.
+
+Definition tm_fv_list t := proj_tm fv_list t.
+Definition fmla_fv_list f := proj_fmla fv_list f.
+
+
+Lemma aset_mem_dec_list {A} `{countable.Countable A} eq_dec x (l: list A):
+  proj_sumbool _ _ (aset_mem_dec x (list_to_aset l)) = in_bool eq_dec x l.
+Proof.
+  destruct (aset_mem_dec _ _); simpl_set; destruct (in_bool_spec eq_dec x l); simpl; auto; simpl_set;
+  try contradiction. rewrite aset_mem_list_to_aset in n; contradiction.
+Qed.
+
+Lemma tm_fv_list_in v t:
+  proj_sumbool _ _ (aset_mem_dec v (tm_fv t)) = in_bool vsymbol_eq_dec v (tm_fv' t).
+Proof.
+  rewrite (tm_fv_list t).
+  apply aset_mem_dec_list.
+Qed.
+
+Lemma fmla_fv_list_in v t:
+  proj_sumbool _ _ (aset_mem_dec v (fmla_fv t)) = in_bool vsymbol_eq_dec v (fmla_fv' t).
+Proof.
+  rewrite (fmla_fv_list t).
+  apply aset_mem_dec_list.
+Qed.
+
+End Fv.
+
+(*Substitution*)
+
+Section Sub.
+
+Definition remove_bindings (subs: list (vsymbol * term)) (vs: list vsymbol) :=
+  filter (fun x => negb (in_dec vsymbol_eq_dec (fst x) vs)) subs.
+
+Definition remove_binding subs v :=
+  remove_bindings subs [v].
+
+
+Fixpoint sub_ts' (subs : list (vsymbol * term)) (t : term) : term :=
+  match t with
+  | Tconst c => Tconst c
+  | Tvar v => match get_assoc_list vsymbol_eq_dec subs v with
+              | Some t1 => t1
+              | None => Tvar v
+              end
+  | Tfun fs tys tms => Tfun fs tys (List.map (sub_ts' subs) tms)
+  | Tlet tm1 v tm2 => Tlet (sub_ts' subs tm1) v (sub_ts' (remove_binding subs v) tm2)
+  | Tif f1 tm1 tm2 => Tif (sub_fs' subs f1) (sub_ts' subs tm1) (sub_ts' subs tm2)
+  | Tmatch tm ty ps =>
+      Tmatch (sub_ts' subs tm) ty
+        (List.map (fun p : pattern * term => (fst p, sub_ts' (remove_bindings subs (pat_fv' (fst p))) (snd p))) ps)
+  | Teps f1 v => Teps (sub_fs' (remove_binding subs v) f1) v
+  end
+with sub_fs' (subs : list (vsymbol * term)) (f : formula) {struct f} : formula :=
+  match f with
+  | Fpred p tys tms => Fpred p tys (List.map (sub_ts' subs) tms)
+  | Fquant q v f' => Fquant q v (sub_fs' (remove_binding subs v) f')
+  | Feq ty tm1 tm2 => Feq ty (sub_ts' subs tm1) (sub_ts' subs tm2)
+  | Fbinop b f1 f2 => Fbinop b (sub_fs' subs f1) (sub_fs' subs f2)
+  | Fnot f' => Fnot (sub_fs' subs f')
+  | Ftrue => Ftrue
+  | Ffalse => Ffalse
+  | Flet tm v f' => Flet (sub_ts' subs tm) v (sub_fs' (remove_binding subs v) f')
+  | Fif f1 f2 f3 => Fif (sub_fs' subs f1) (sub_fs' subs f2) (sub_fs' subs f3)
+  | Fmatch tm ty ps =>
+      Fmatch (sub_ts' subs tm) ty
+        (List.map (fun p : pattern * formula => ((fst p), sub_fs' (remove_bindings subs (pat_fv' (fst p))) (snd p)))
+           ps)
+  end.
+
+Lemma get_assoc_list_irrel {A B} (eq1 eq2: forall (x y: A), {x = y} + {x <> y}) (l: list (A * B)) (x: A):
+  get_assoc_list eq1 l x = get_assoc_list eq2 l x.
+Proof.
+  induction l as [| h t IH]; simpl; auto.
+  destruct (eq1 x (fst h)); destruct (eq2 x (fst h)); subst; simpl; try contradiction; auto.
+Qed.
+
+Lemma remove_bindings_notin subs vs v:
+  In v vs ->
+  ~ In v (map fst (remove_bindings subs vs)).
+Proof.
+  intros. induction subs; simpl in *; auto.
+  destruct (in_dec vsymbol_eq_dec (fst a) vs); simpl; auto.
+  intro C. destruct C; subst; auto.
+Qed.
+
+(*This direction is OK bc we have extensionality*)
+Lemma remove_bindings_list l s:
+  SubMulti.remove_bindings (list_to_amap l) (list_to_aset s) =
+  list_to_amap (remove_bindings l s).
+Proof.
+  apply amap_ext. intros x.
+  rewrite remove_bindings_eq.
+  destruct (aset_mem_dec x (list_to_aset s)) as [Hxs | Hxs]; simpl_set.
+  - rewrite amap_diff_in; simpl_set; auto. symmetry; apply list_to_amap_none.
+    apply remove_bindings_notin; auto.
+  - rewrite amap_diff_notin; auto.
+    (*avoid nodup hyp*)
+    induction l as [| h t IH]; simpl; auto.
+    rewrite aset_mem_list_to_aset in Hxs.
+    destruct (in_dec vsymbol_eq_dec (fst h) s) as [Hsh | Hsh]; simpl; auto.
+    + rewrite amap_set_lookup_diff; auto. intro C; subst; contradiction.
+    + vsym_eq x (fst h); try contradiction.
+      * rewrite !amap_set_lookup_same; auto.
+      * rewrite !amap_set_lookup_diff; auto.
+Qed.
+
+
+Lemma remove_binding_list l v:
+  SubMulti.remove_binding (list_to_amap l) v = list_to_amap (remove_binding l v).
+Proof.
+  apply amap_ext. intros x.
+  rewrite remove_binding_eq.
+  vsym_eq x v.
+  - rewrite amap_remove_same. symmetry. apply list_to_amap_none.
+    apply remove_bindings_notin. simpl; auto.
+  - rewrite amap_remove_diff; auto.
+    (*avoid nodup hyp*)
+    induction l as [| h t IH]; simpl; auto.
+    vsym_eq v (fst h); simpl; auto.
+    + rewrite amap_set_lookup_diff; auto.
+    + vsym_eq x (fst h); try contradiction.
+      * rewrite !amap_set_lookup_same; auto.
+      * rewrite !amap_set_lookup_diff; auto.
+Qed.
+
+(*Prove equal*)
+Lemma sub_equiv t f:
+  (forall l, sub_ts (list_to_amap l) t = sub_ts' l t) /\
+  (forall l, sub_fs (list_to_amap l) f = sub_fs' l f).
+Proof.
+  revert t f; apply term_formula_ind; simpl; auto.
+  - intros v l. rewrite amap_lookup_list.
+    erewrite get_assoc_list_irrel. reflexivity.
+  - intros f tys tms IH l. f_equal.
+    apply list_eq_ext'; simpl_len; auto. intros n d Hn.
+    rewrite -> !map_nth_inbound with (d2:=tm_d); auto.
+    rewrite Forall_nth in IH. apply IH; auto.
+  - intros tm1 v tm2 IH1 IH2 l. rewrite -> IH1. f_equal.
+    rewrite remove_binding_list. apply IH2.
+  - intros f t1 t2 IH1 IH2 IH3 l. rewrite -> IH1, IH2, IH3; auto.
+  - intros tm ty ps IH1 IH2 l. rewrite IH1. f_equal.
+    rewrite Forall_map in IH2. apply list_eq_ext'; simpl_len; auto.
+    intros n d Hn. rewrite -> !map_nth_inbound with (d2:=(Pwild, tm_d)); auto.
+    f_equal. rewrite -> pat_fv_list, remove_bindings_list. 
+    rewrite Forall_nth in IH2. apply IH2; auto.
+  - intros f v IH l. rewrite remove_binding_list. f_equal; apply IH.
+  - intros p tys tms IH l. f_equal.
+    apply list_eq_ext'; simpl_len; auto. intros n d Hn.
+    rewrite -> !map_nth_inbound with (d2:=tm_d); auto.
+    rewrite Forall_nth in IH. apply IH; auto.
+  - intros q v f IH l. f_equal. rewrite remove_binding_list. apply IH.
+  - intros ty t1 t2 IH1 IH2 l. rewrite -> IH1, IH2; reflexivity.
+  - intros b f1 f2 IH1 IH2 l. rewrite -> IH1, IH2; reflexivity.
+  - intros f IH l. f_equal; apply IH.
+  - intros tm v f IH1 IH2 l. rewrite -> IH1. f_equal.
+    rewrite remove_binding_list. apply IH2.
+  - intros f1 f2 f3 IH1 IH2 IH3 l. rewrite -> IH1, IH2, IH3; auto.
+  - intros tm ty ps IH1 IH2 l. rewrite IH1. f_equal.
+    rewrite Forall_map in IH2. apply list_eq_ext'; simpl_len; auto.
+    intros n d Hn. rewrite -> !map_nth_inbound with (d2:=(Pwild, Ftrue)); auto.
+    f_equal. rewrite -> pat_fv_list, remove_bindings_list. 
+    rewrite Forall_nth in IH2. apply IH2; auto.
+Qed.
+
+Definition sub_ts_equiv l t:= proj_tm sub_equiv t l.
+Definition sub_fs_equiv l f:=proj_fmla sub_equiv f l.
+
+
+(*NOTE: lots of this breaks/does not compute well if I actually need alpha conversion*)
+(*Can use [list_to_amap] in set because we will vm_compute to bool anyway*)
+Definition safe_sub_ts' (subs: (list (vsymbol * term))) (t: term) : term :=
+  (*TODO: bad, would be nice to have proper computable but tricky*)
+  if check_disj (aset_big_union tm_fv (vals (list_to_amap subs))) (list_to_aset (tm_bnd t)) then
+  sub_ts' subs t else
+  sub_ts' subs (a_convert_t t (aset_big_union tm_fv (vals (list_to_amap subs)))).
+
+Lemma safe_sub_ts_equiv subs t:
+  safe_sub_ts' subs t =
+  safe_sub_ts (list_to_amap subs) t.
+Proof.
+  unfold safe_sub_ts', safe_sub_ts.
+  destruct (check_disj _ _);  symmetry; apply sub_ts_equiv.
+Qed.
+
+Definition safe_sub_fs' (subs: (list (vsymbol * term))) (f: formula) : formula :=
+  if check_disj (aset_big_union tm_fv (vals (list_to_amap subs))) (list_to_aset (fmla_bnd f)) then
+  sub_fs' subs f else
+  sub_fs' subs (a_convert_f f (aset_big_union tm_fv (vals (list_to_amap subs)))).
+
+Lemma safe_sub_fs_equiv subs f:
+  safe_sub_fs' subs f =
+  safe_sub_fs (list_to_amap subs) f.
+Proof.
+  unfold safe_sub_fs', safe_sub_fs.
+  destruct (check_disj _ _);  symmetry; apply sub_fs_equiv.
+Qed.
+
+End Sub.
+
+
+(*The main pieces: [simpl_match] and rewriting*)
+
+(*Redo part of [simpl_match]*)
+Section MatchSimpl'.
+
+Import MatchSimpl.
+
+Inductive match_result : Type :=
+  | DontKnow : match_result
+  | NoMatch : match_result
+  | Matches : list (vsymbol * term) -> match_result.
+
+Fixpoint matches gamma (p: pattern) (t: term) : match_result :=
+  match p, t with
+  | Pvar x, _ => Matches [(x, t)]
+  | Pwild, _ => Matches nil
+  | Por p1 p2, _ => 
+    match (matches gamma p1 t) with
+    | NoMatch => matches gamma p2 t
+    | r => r
+    end
+  | Pbind p1 x, _ => match (matches gamma p1 t) with
+                  | Matches l => Matches ((x, t) :: l)
+                  | r => r
+                  end
+  | Pconstr f1 tys1 ps, Tfun f2 tys2 tms =>
+    if funsym_eq_dec f1 f2 && list_eq_dec vty_eq_dec tys1 tys2 &&
+      (Nat.eqb (length ps) (length tms)) then
+    (fix nested_matches (p1: list pattern) (t1: list term) : match_result :=
+      match p1, t1 with
+      | p :: ps, t :: ts => 
+        match matches gamma p t, nested_matches ps ts with
+        | Matches l1, Matches l2 => Matches (l1 ++ l2)
+        | DontKnow, _ => DontKnow
+        | _, DontKnow => DontKnow
+        | _, _ => NoMatch
+        end
+      | nil, nil => Matches nil
+      | _, _ => (*Impossible*) DontKnow
+      end) ps tms
+    else
+    if (is_funsym_constr gamma f2) then NoMatch
+    else DontKnow
+  | Pconstr _ _ _, Tconst _ => NoMatch
+  | Pconstr _ _ _, _ => DontKnow
+  end.
+
+(*rewrite lemma*)
+Fixpoint nested_matches gamma (ps: list pattern) (ts: list term) : match_result :=
+  match ps, ts with
+    | p :: ps, t :: ts => 
+      match matches gamma p t, nested_matches gamma ps ts with
+      | Matches l1, Matches l2 => Matches (l1 ++ l2)
+      | DontKnow, _ => DontKnow
+      | _, DontKnow => DontKnow
+      | _, _ => NoMatch
+      end
+    | nil, nil => Matches nil
+    | _, _ => (*Impossible*) DontKnow
+  end.
+
+Lemma matches_constr_rewrite gamma f1 tys1 ps1 t:
+  matches gamma (Pconstr f1 tys1 ps1) t =
+  match t with
+  | Tfun f2 tys2 tms =>
+     if funsym_eq_dec f1 f2 && list_eq_dec vty_eq_dec tys1 tys2 &&
+      (length ps1 =? length tms) then
+      nested_matches gamma ps1 tms
+    else if (is_funsym_constr gamma f2) then NoMatch
+    else DontKnow
+  | Tconst c => NoMatch
+  | _ => DontKnow
+  end.
+Proof.
+  simpl. destruct t; auto.
+  destruct (funsym_eq_dec f1 f); auto; simpl; subst.
+  destruct (list_eq_dec vty_eq_dec tys1 l); auto; simpl; subst.
+  destruct (Nat.eqb_spec (length ps1) (length l0)); auto.
+  generalize dependent l0. induction ps1; simpl; intros; auto.
+  destruct l0; auto.
+  destruct (matches gamma a t) eqn : Hmatch; auto;
+  rewrite IHps1; auto.
+Qed.
+
+Fixpoint check_match (gamma: context) {A: Type} (sub: list (vsymbol * term) -> A -> A)
+(t: term) (ret: A) (l: list (pattern * A)) : A :=
+match l with
+| nil => ret
+| pt :: tl => 
+  match (matches gamma (fst pt) t) with
+  | NoMatch => check_match gamma sub t ret tl
+  | DontKnow => ret
+  | Matches subs => sub subs (snd pt)
+  end
+end.
+
+Definition match_result_eq (m: match_result) (m2: MatchSimpl.match_result) : Prop :=
+  match m, m2 with
+  | DontKnow, MatchSimpl.DontKnow => True
+  | NoMatch, MatchSimpl.NoMatch => True
+  | Matches l, MatchSimpl.Matches m => list_to_amap l = m
+  | _, _ => False
+  end.
+
+
+Opaque amap_singleton list_to_amap.
+Lemma matches_eq gamma p t:
+  match_result_eq (matches gamma p t) (MatchSimpl.matches gamma p t).
+Proof.
+  revert t.
+  induction p as [v | f tys ps IH | | q1 q2 IH1 IH2 | p v IH]; intros t.
+  - simpl. symmetry; apply amap_singleton_list.
+  - rewrite -> matches_constr_rewrite, MatchSimpl.matches_constr_rewrite.
+    destruct t as [| | f1 tys1 tms | | | | ]; try solve[unfold match_result_eq; auto].
+    destruct (funsym_eq_dec f f1); subst; simpl; auto.
+    2: { destruct (is_funsym_constr gamma f1); reflexivity. }
+    destruct (list_eq_dec vty_eq_dec tys tys1); subst; simpl; auto.
+    2: { destruct (is_funsym_constr gamma f1); reflexivity. }
+    destruct (Nat.eqb_spec (length ps) (length tms)) as [Hlen | Hlen]; simpl; auto.
+    2: { destruct (is_funsym_constr gamma f1); reflexivity. }
+    generalize dependent tms. induction ps as [| p1 ptl IHp];
+    intros [| t1 ttl]; try discriminate; auto; simpl.
+    + intros; reflexivity.
+    + intros Hlen.
+      inversion IH as [| ? ? IH1 IH2]; clear IH; subst.
+      specialize (IH1 t1). specialize (IHp IH2 ttl ltac:(auto)). clear IH2.
+      unfold match_result_eq in IH1.
+      destruct (matches gamma p1 t1) eqn : Hmatch1;
+      destruct (MatchSimpl.matches gamma p1 t1) eqn: Hmatch2; auto; try contradiction.
+      * unfold match_result_eq in IHp.
+        destruct (nested_matches gamma ptl ttl) eqn : Hmatch3; 
+        destruct (MatchSimpl.nested_matches gamma ptl ttl) eqn : Hmatch4; auto.
+      * unfold match_result_eq in IHp.
+        destruct (nested_matches gamma ptl ttl) eqn : Hmatch3; 
+        destruct (MatchSimpl.nested_matches gamma ptl ttl) eqn : Hmatch4; auto.
+        unfold match_result_eq. subst. 
+        apply amap_union_list.
+  - simpl. reflexivity.
+  - simpl. specialize (IH1 t). specialize (IH2 t). unfold match_result_eq in *.
+    destruct (matches gamma q1 t); destruct (MatchSimpl.matches gamma q1 t); auto;
+    contradiction.
+  - simpl. specialize (IH t). unfold match_result_eq in *.
+    destruct (matches gamma p t); destruct (MatchSimpl.matches gamma p); auto;
+    try contradiction. subst. reflexivity.
+Qed.
+
+Lemma check_match_eq gamma {A: Type} (sub1: list (vsymbol * term) -> A -> A)
+  (sub2: amap vsymbol term -> A -> A)
+  t ret l (Hsub: forall l x, sub2 (list_to_amap l) x = sub1 l x):
+  check_match gamma sub1 t ret l =
+  MatchSimpl.check_match gamma sub2 t ret l.
+Proof.
+  induction l as [| h tl IH]; simpl; auto.
+  pose proof (matches_eq gamma (fst h) t) as Hmatch.
+  unfold match_result_eq in Hmatch.
+  destruct (matches gamma (fst h) t); destruct ( MatchSimpl.matches gamma (fst h) t); auto; try contradiction.
+  subst. auto.
+Qed.
+
+Lemma check_match_sub_eq gamma t ret l:
+  MatchSimpl.check_match gamma safe_sub_ts t ret l =
+  check_match gamma safe_sub_ts' t ret l.
+Proof.
+  symmetry; apply check_match_eq.
+  intros; symmetry; apply safe_sub_ts_equiv.
+Qed.
+
+Lemma check_match_sub_eq' gamma t ret l:
+  MatchSimpl.check_match gamma safe_sub_fs t ret l =
+  check_match gamma safe_sub_fs' t ret l.
+Proof.
+  symmetry; apply check_match_eq.
+  intros; symmetry; apply safe_sub_fs_equiv.
+Qed.
+
+Fixpoint simpl_match_t gamma (t: term) : term :=
+  match t with
+  | Tfun f tys tms => Tfun f tys (map (simpl_match_t gamma) tms)
+  | Tlet t1 x t2 => Tlet (simpl_match_t gamma t1) x (simpl_match_t gamma t2)
+  | Tif f1 t1 t2 => Tif (simpl_match_f gamma f1) (simpl_match_t gamma t1) (simpl_match_t gamma t2)
+  | Tmatch t1 ty ps =>
+    check_match gamma safe_sub_ts' t1 t ps
+  | Teps f x => Teps (simpl_match_f gamma f) x
+  | _ => t
+  end
+with simpl_match_f gamma (f: formula) : formula :=
+  match f with
+  | Fpred p tys tms => Fpred p tys (map (simpl_match_t gamma) tms)
+  | Fquant q x f => Fquant q x (simpl_match_f gamma f)
+  | Feq ty t1 t2 => Feq ty (simpl_match_t gamma t1) (simpl_match_t gamma t2)
+  | Fbinop b f1 f2 => Fbinop b (simpl_match_f gamma f1) (simpl_match_f gamma f2)
+  | Flet t x f => Flet (simpl_match_t gamma t) x (simpl_match_f gamma f)
+  | Fif f1 f2 f3 => Fif (simpl_match_f gamma f1) (simpl_match_f gamma f2) (simpl_match_f gamma f3)
+  | Fmatch t1 ty ps =>
+    check_match gamma safe_sub_fs' t1 f ps
+  | _ => f
+  end.
+
+Lemma simpl_match_eq gamma t f:
+  (simpl_match_t gamma t = MatchSimpl.simpl_match_t gamma t) /\
+  (simpl_match_f gamma f = MatchSimpl.simpl_match_f gamma f).
+Proof.
+  revert t f; apply term_formula_ind; simpl; auto.
+  - intros f tys tms IH. f_equal. 
+    apply list_eq_ext'; simpl_len; auto. intros n' d Hn.
+    rewrite !map_nth_inbound with (d2:=tm_d); auto. rewrite Forall_nth in IH; auto.
+  - intros ? ? ? IH1 IH2. rewrite IH1, IH2; reflexivity.
+  - intros ? ? ? IH1 IH2 IH3. rewrite IH1, IH2, IH3; reflexivity.
+  - intros. symmetry; apply check_match_sub_eq.
+  - intros ? ? IH. rewrite IH; reflexivity.
+  - intros ? ? ? IH. f_equal. 
+    apply list_eq_ext'; simpl_len; auto. intros n' d Hn.
+    rewrite !map_nth_inbound with (d2:=tm_d); auto. rewrite Forall_nth in IH; auto.
+  - intros ? ? ? IH; rewrite IH; reflexivity.
+  - intros ? ? ? IH1 IH2; rewrite IH1, IH2; reflexivity.
+  - intros ? ? ? IH1 IH2; rewrite IH1, IH2; reflexivity.
+  - intros ? ? ? IH1 IH2. rewrite IH1, IH2; reflexivity.
+  - intros ? ? ? IH1 IH2 IH3. rewrite IH1, IH2, IH3; reflexivity.
+  - intros. symmetry; apply check_match_sub_eq'.
+Qed.
+
+Definition simpl_match_t_eq gamma t := proj_tm (simpl_match_eq gamma) t.
+Definition simpl_match_f_eq gamma f := proj_fmla (simpl_match_eq gamma) f.
+
+End MatchSimpl'.
+
+(*And for rewrite/unfold*)
+Section Replace.
+Variable tm_o tm_n: term.
+
+Fixpoint replace_tm_t (t: term) :=
+  if term_eq_dec tm_o t then tm_n else
+  (*Just a bunch of recursive cases*)
+  match t with
+  | Tfun f tys tms => Tfun f tys (map replace_tm_t tms)
+  | Tlet t1 v t2 =>
+    Tlet (replace_tm_t t1) v 
+    (*Avoid capture -*)
+    (if in_bool vsymbol_eq_dec v (tm_fv' tm_o) then t2
+    else (replace_tm_t t2))
+  | Tif f t1 t2 =>
+    Tif (replace_tm_f f) (replace_tm_t t1) (replace_tm_t t2)
+  | Tmatch tm ty ps =>
+    Tmatch (replace_tm_t tm) ty
+    (map (fun x => (fst x, 
+      if existsb (fun v => in_bool vsymbol_eq_dec v (tm_fv' tm_o))
+       (pat_fv' (fst x))
+         then
+      snd x else (replace_tm_t (snd x)))) ps)
+  | Teps f v =>
+    Teps (if in_bool vsymbol_eq_dec v (tm_fv' tm_o) then f else
+      replace_tm_f f) v
+  | _ => t
+  end
+with replace_tm_f (f: formula) :=
+  match f with
+  | Fpred p tys tms =>
+    Fpred p tys (map replace_tm_t tms)
+  | Fquant q v f =>
+    Fquant q v (if in_bool vsymbol_eq_dec v (tm_fv' tm_o) then f else
+      replace_tm_f f)
+  | Feq ty t1 t2 => Feq ty (replace_tm_t t1) (replace_tm_t t2)
+  | Fbinop b f1 f2 => Fbinop b (replace_tm_f f1) (replace_tm_f f2)
+  | Fnot f => Fnot (replace_tm_f f)
+  | Flet t v f => Flet (replace_tm_t t) v
+    (if in_bool vsymbol_eq_dec v (tm_fv' tm_o) then f 
+      else (replace_tm_f f))
+  | Fif f1 f2 f3 => Fif (replace_tm_f f1) (replace_tm_f f2)
+    (replace_tm_f f3)
+  | Fmatch tm ty ps =>
+    Fmatch (replace_tm_t tm) ty
+    (map (fun x => (fst x, 
+      if existsb (fun v => in_bool vsymbol_eq_dec v (tm_fv' tm_o))
+      (pat_fv' (fst x))
+        then
+      snd x else (replace_tm_f (snd x)))) ps)
+  | _ => f
+  end.
+
+(*For patmatch case*)
+Lemma existsb_pat_fv_list p t:
+   existsb (fun v : vsymbol => aset_mem_dec v (tm_fv t))
+      (aset_to_list (pat_fv p)) =
+    existsb (fun v : vsymbol => in_bool vsymbol_eq_dec v (tm_fv' t))
+      (pat_fv' p).
+Proof.
+  apply is_true_eq. unfold is_true. rewrite !existsb_exists.
+  setoid_rewrite pat_fv_list. split.
+  - intros [v [Hinv Hfv]]. simpl_set. exists v; split; auto.
+    erewrite tm_fv_list, aset_mem_dec_list in Hfv. apply Hfv.
+  - intros [v [Hinv Hfv]]. exists v. simpl_set. split; auto.
+    erewrite tm_fv_list, aset_mem_dec_list. apply Hfv.
+Qed.
+
+Lemma replace_tm_eq t f:
+  (Rewrite.replace_tm_t tm_o tm_n t = replace_tm_t t) /\
+  (Rewrite.replace_tm_f tm_o tm_n f = replace_tm_f f).
+Proof.
+  revert t f; apply term_formula_ind; simpl; try reflexivity.
+  - intros f tys tms IH. destruct (term_eq_dec tm_o (Tfun f tys tms)); auto.
+    f_equal. apply list_eq_ext'; simpl_len; auto. intros n' d Hn.
+    rewrite !map_nth_inbound with (d2:=tm_d); auto. rewrite Forall_nth in IH; auto.
+  - intros tm1 v tm2 IH1 IH2. destruct (term_eq_dec _ _); auto.
+    rewrite IH1. f_equal. rewrite <- tm_fv_list_in. destruct (aset_mem_dec _ _); auto.
+  - intros f t1 t2 IH1 IH2 IH3. destruct (term_eq_dec _ _); auto.
+    rewrite IH1, IH2, IH3; reflexivity.
+  - intros tm ty ps IH IHps. destruct (term_eq_dec _ _); auto.
+    rewrite IH; f_equal. clear IH n. rewrite Forall_map in IHps.
+    apply list_eq_ext'; simpl_len; auto. intros n' d Hn.
+    rewrite !map_nth_inbound with (d2:=(Pwild, tm_d)); auto.
+    f_equal. rewrite existsb_pat_fv_list. destruct (existsb _ _); auto.
+    rewrite Forall_nth in IHps. auto.
+  - intros f v IH. destruct (term_eq_dec _ _); auto.
+    rewrite <- tm_fv_list_in. destruct (aset_mem_dec _ _); simpl; auto. f_equal; auto.
+  - intros p tys tms IH.
+    f_equal. apply list_eq_ext'; simpl_len; auto. intros n' d Hn.
+    rewrite !map_nth_inbound with (d2:=tm_d); auto. rewrite Forall_nth in IH; auto.
+  - intros q f v IH. rewrite <- tm_fv_list_in. destruct (aset_mem_dec _ _); simpl; auto. f_equal; auto.
+  - intros ty t1 t2 IH1 IH2. rewrite IH1, IH2; reflexivity.
+  - intros b t1 t2 IH1 IH2. rewrite IH1, IH2; reflexivity.
+  - intros f IH. rewrite IH; reflexivity.
+  - intros tm1 v tm2 IH1 IH2.
+    rewrite IH1. f_equal. rewrite <- tm_fv_list_in. destruct (aset_mem_dec _ _); auto.
+  - intros f t1 t2 IH1 IH2 IH3. rewrite IH1, IH2, IH3; reflexivity.
+  - intros tm ty ps IH IHps. 
+    rewrite IH; f_equal. clear IH. rewrite Forall_map in IHps.
+    apply list_eq_ext'; simpl_len; auto. intros n' d Hn.
+    rewrite !map_nth_inbound with (d2:=(Pwild, Ftrue)); auto.
+    f_equal. rewrite existsb_pat_fv_list. destruct (existsb _ _); auto.
+    rewrite Forall_nth in IHps. auto.
+Qed.
+
+Definition replace_tm_t_eq t := proj_tm replace_tm_eq t.
+Definition replace_tm_f_eq f := proj_fmla replace_tm_eq f.
+
+End Replace.
+
+(*And replace fmla*)
+Section ReplaceFmla.
+
+Variable fmla_o fmla_n: formula.
+
+Fixpoint replace_fmla_t (t: term) :=
+  (*Just a bunch of recursive cases*)
+  match t with
+  | Tfun f tys tms => Tfun f tys (map replace_fmla_t tms)
+  | Tlet t1 v t2 =>
+    Tlet (replace_fmla_t t1) v 
+    (*Avoid capture -*)
+    (if in_bool vsymbol_eq_dec v (fmla_fv' fmla_o) then t2
+    else (replace_fmla_t t2))
+  | Tif f t1 t2 =>
+    Tif (replace_fmla_f f) (replace_fmla_t t1) (replace_fmla_t t2)
+  | Tmatch tm ty ps =>
+    Tmatch (replace_fmla_t tm) ty
+    (map (fun x => (fst x, 
+      if existsb (fun v => in_bool vsymbol_eq_dec v (fmla_fv' fmla_o))
+       (pat_fv' (fst x))
+         then
+      snd x else (replace_fmla_t (snd x)))) ps)
+  | Teps f v =>
+    Teps (if in_bool vsymbol_eq_dec v (fmla_fv' fmla_o) then f else
+    replace_fmla_f f) v
+  | _ => t
+  end
+with replace_fmla_f (f: formula) :=
+if formula_eq_dec fmla_o f then fmla_n else
+  match f with
+  | Fpred p tys tms =>
+    Fpred p tys (map replace_fmla_t tms)
+  | Fquant q v f =>
+    Fquant q v (if in_bool vsymbol_eq_dec v (fmla_fv' fmla_o) then f else
+    replace_fmla_f f)
+  | Feq ty t1 t2 => Feq ty (replace_fmla_t t1) (replace_fmla_t t2)
+  | Fbinop b f1 f2 => Fbinop b (replace_fmla_f f1) (replace_fmla_f f2)
+  | Fnot f => Fnot (replace_fmla_f f)
+  | Flet t v f => Flet (replace_fmla_t t) v
+    (if in_bool vsymbol_eq_dec v (fmla_fv' fmla_o) then f 
+      else (replace_fmla_f f))
+  | Fif f1 f2 f3 => Fif (replace_fmla_f f1) (replace_fmla_f f2)
+    (replace_fmla_f f3)
+  | Fmatch tm ty ps =>
+    Fmatch (replace_fmla_t tm) ty
+    (map (fun x => (fst x, 
+      if existsb (fun v => in_bool vsymbol_eq_dec v (fmla_fv' fmla_o))
+      (pat_fv' (fst x))
+        then
+      snd x else (replace_fmla_f (snd x)))) ps)
+  | _ => f
+  end.
+
+Lemma existsb_pat_fv_list' p t:
+   existsb (fun v : vsymbol => aset_mem_dec v (fmla_fv t))
+      (aset_to_list (pat_fv p)) =
+    existsb (fun v : vsymbol => in_bool vsymbol_eq_dec v (fmla_fv' t))
+      (pat_fv' p).
+Proof.
+  apply is_true_eq. unfold is_true. rewrite !existsb_exists.
+  setoid_rewrite pat_fv_list. split.
+  - intros [v [Hinv Hfv]]. simpl_set. exists v; split; auto.
+    erewrite fmla_fv_list, aset_mem_dec_list in Hfv. apply Hfv.
+  - intros [v [Hinv Hfv]]. exists v. simpl_set. split; auto.
+    erewrite fmla_fv_list, aset_mem_dec_list. apply Hfv.
+Qed.
+
+
+Lemma replace_fmla_eq t f:
+  (Rewrite.replace_fmla_t fmla_o fmla_n t = replace_fmla_t t) /\
+  (Rewrite.replace_fmla_f fmla_o fmla_n f = replace_fmla_f f).
+Proof.
+  revert t f; apply term_formula_ind; simpl; try reflexivity.
+  - intros f tys tms IH. f_equal. apply list_eq_ext'; simpl_len; auto. intros n' d Hn.
+    rewrite !map_nth_inbound with (d2:=tm_d); auto. rewrite Forall_nth in IH; auto.
+  - intros tm1 v tm2 IH1 IH2. 
+    rewrite IH1. f_equal. rewrite <- fmla_fv_list_in. destruct (aset_mem_dec _ _); auto.
+  - intros f t1 t2 IH1 IH2 IH3. rewrite IH1, IH2, IH3; reflexivity.
+  - intros tm ty ps IH IHps. rewrite IH; f_equal. clear IH. rewrite Forall_map in IHps.
+    apply list_eq_ext'; simpl_len; auto. intros n' d Hn.
+    rewrite !map_nth_inbound with (d2:=(Pwild, tm_d)); auto.
+    f_equal. rewrite existsb_pat_fv_list'. destruct (existsb _ _); auto.
+    rewrite Forall_nth in IHps. auto.
+  - intros f v IH. rewrite <- fmla_fv_list_in. destruct (aset_mem_dec _ _); simpl; auto. f_equal; auto.
+  - intros p tys tms IH. destruct (formula_eq_dec _ _); auto.
+    f_equal. apply list_eq_ext'; simpl_len; auto. intros n' d Hn.
+    rewrite !map_nth_inbound with (d2:=tm_d); auto. rewrite Forall_nth in IH; auto.
+  - intros q f v IH. destruct (formula_eq_dec _ _); auto. 
+    rewrite <- fmla_fv_list_in. destruct (aset_mem_dec _ _); simpl; auto. f_equal; auto.
+  - intros ty t1 t2 IH1 IH2. destruct (formula_eq_dec _ _); auto. rewrite IH1, IH2; reflexivity.
+  - intros b t1 t2 IH1 IH2. destruct (formula_eq_dec _ _); auto. rewrite IH1, IH2; reflexivity.
+  - intros f IH. destruct (formula_eq_dec _ _); auto. rewrite IH; reflexivity.
+  - intros tm1 v tm2 IH1 IH2. destruct (formula_eq_dec _ _); auto.
+    rewrite IH1. f_equal. rewrite <- fmla_fv_list_in. destruct (aset_mem_dec _ _); auto.
+  - intros f t1 t2 IH1 IH2 IH3. destruct (formula_eq_dec _ _); auto. rewrite IH1, IH2, IH3; reflexivity.
+  - intros tm ty ps IH IHps. destruct (formula_eq_dec _ _); auto. 
+    rewrite IH; f_equal. clear IH. rewrite Forall_map in IHps.
+    apply list_eq_ext'; simpl_len; auto. intros n' d Hn.
+    rewrite !map_nth_inbound with (d2:=(Pwild, Ftrue)); auto.
+    f_equal. rewrite existsb_pat_fv_list'. destruct (existsb _ _); auto.
+    rewrite Forall_nth in IHps. auto.
+Qed.
+
+Definition replace_fmla_t_eq t := proj_tm replace_fmla_eq t.
+Definition replace_fmla_f_eq f := proj_fmla replace_fmla_eq f.
+
+End ReplaceFmla.
